src/3d/Target.fsti
@@ -421,7 +421,9 @@ val print_decls (modul: string) (ds:list decl) : ML string
 val print_types_decls (modul: string) (ds:list decl) : ML string
 val print_decls_signature (modul: string) (ds:list decl) : ML string
 val wrapper_name (modul: string) (fn: string) : ML string
-val print_c_entry (modul: string) (env: global_env) (ds:list decl)
+type produce_everparse_error = | ProduceEverParseError
+type opt_produce_everparse_error = option produce_everparse_error
+val print_c_entry (_: opt_produce_everparse_error) (modul: string) (env: global_env) (ds:list decl)
   : ML (string & string)
 
 (*
